feat: NormalEq is transitive :tada:

Lean4Lean/Theory/Typing/ParallelReduction.lean
@@ -89,35 +89,64 @@ theorem ParRed.instN (W : Ctx.InstN Γ₀ a1 A₀ k Γ₁ Γ)
     obtain ⟨_, _, h', rfl, rfl⟩ := HE.2 W h
     exact ih _ _ h' W
 
+variable (IsDefEq : List VExpr → VExpr → VExpr → Prop) (Γ₀ : List VExpr) in
+inductive IsDefEqCtx : List VExpr → List VExpr → Prop
+  | zero : IsDefEqCtx Γ₀ Γ₀
+  | succ : IsDefEqCtx Γ₁ Γ₂ → IsDefEq Γ₁ A₁ A₂ → IsDefEqCtx (A₁ :: Γ₁) (A₂ :: Γ₂)
+
 section
 set_option hygiene false
 local notation:65 Γ " ⊢ " e " : " A:36 => HasType Γ e A
 local notation:65 Γ " ⊢ " e1 " ≡ " e2:36 => IsDefEq Γ e1 e2
 structure Typing where
+  env : VEnv
+  -- henv : env.Ordered
   univs : Nat
   IsDefEq : List VExpr → VExpr → VExpr → Prop
   HasType : List VExpr → VExpr → VExpr → Prop
   refl : Γ ⊢ e : A → Γ ⊢ e ≡ e
   symm : Γ ⊢ e₁ ≡ e₂ → Γ ⊢ e₂ ≡ e₁
   trans : Γ ⊢ e₁ ≡ e₂ → Γ ⊢ e₂ ≡ e₃ → Γ ⊢ e₁ ≡ e₃
+  bvar : Lookup Γ i A → Γ ⊢ .bvar i : A
   sort : u.WF univs → Γ ⊢ .sort u : .sort u.succ
   sortDF : u.WF univs → v.WF univs → u ≈ v → Γ ⊢ .sort u ≡ .sort v
+  constDF :
+    env.constants c = some (some ci) →
+    (∀ l ∈ ls, l.WF univs) → (∀ l ∈ ls', l.WF univs) →
+    ls.length = ci.uvars → List.Forall₂ (· ≈ ·) ls ls' →
+    Γ ⊢ .const c ls ≡ .const c ls'
   appDF : Γ ⊢ f : .forallE A B → Γ ⊢ f ≡ f' → Γ ⊢ a : A → Γ ⊢ a ≡ a' → Γ ⊢ .app f a ≡ .app f' a'
   lamDF : Γ ⊢ A : .sort u → Γ ⊢ A ≡ A' → A::Γ ⊢ body ≡ body' → Γ ⊢ .lam A body ≡ .lam A' body'
   forallEDF :
     Γ ⊢ A : .sort u → Γ ⊢ A ≡ A' →
     A::Γ ⊢ body : .sort v → A::Γ ⊢ body ≡ body' →
     Γ ⊢ .forallE A body ≡ .forallE A' body'
+  app : Γ ⊢ f : .forallE A B → Γ ⊢ a : A → Γ ⊢ .app f a : .inst B a
+  lam : Γ ⊢ A : .sort u → A::Γ ⊢ body : B → Γ ⊢ .lam A body : .forallE A B
+  forallE : Γ ⊢ A : .sort u → A::Γ ⊢ B : .sort v → Γ ⊢ .forallE A B : .sort (.imax u v)
   eta : Γ ⊢ e : .forallE A B → Γ ⊢ .lam A (.app e.lift (.bvar 0)) ≡ e
   proofIrrel : Γ ⊢ p : .sort .zero → Γ ⊢ h : p → Γ ⊢ h' : p → Γ ⊢ h ≡ h'
+  isDefEq_weakN_iff (W : Ctx.LiftN n k Γ Γ') :
+    Γ' ⊢ e1.liftN n k ≡ e2.liftN n k ↔ Γ ⊢ e1 ≡ e2
+  hasType_weakN_iff (W : Ctx.LiftN n k Γ Γ') : Γ' ⊢ e.liftN n k : A.liftN n k ↔ Γ ⊢ e : A
+  hasTypeU_weakN_inv (W : Ctx.LiftN n k Γ Γ') : Γ' ⊢ e.liftN n k : A → ∃ A', Γ ⊢ e : A'
+  isDefEq_DFC : IsDefEqCtx IsDefEq Γ₀ Γ₁ Γ₂ → Γ₁ ⊢ e1 ≡ e2 → Γ₂ ⊢ e1 ≡ e2
+  hasType_DFC : IsDefEqCtx IsDefEq Γ₀ Γ₁ Γ₂ → Γ₁ ⊢ e : A → Γ₂ ⊢ e : A
   has_type : Γ ⊢ e₁ ≡ e₂ → ∃ A, Γ ⊢ e₁ : A
   is_type : Γ ⊢ e : A → ∃ u, Γ ⊢ A : .sort u
   sort_inv : Γ ⊢ .sort u : p → u.WF univs
-  forallE_inv : Γ ⊢ .forallE A B : V → ∃ u v, Γ ⊢ A : .sort u ∧ A::Γ ⊢ A : .sort v
+  forallE_inv : Γ ⊢ .forallE A B : V → ∃ u v, Γ ⊢ A : .sort u ∧ A::Γ ⊢ B : .sort v
+  app_inv : Γ ⊢ .app f a : V → ∃ A B, Γ ⊢ f : .forallE A B ∧ Γ ⊢ a : A
   uniq : Γ ⊢ e : A₁ → Γ ⊢ e : A₂ → Γ ⊢ A₁ ≡ A₂
   defeq_l : Γ ⊢ e₁ ≡ e₂ → Γ ⊢ e₁ : A → Γ ⊢ e₂ : A
   defeq_r : Γ ⊢ A₁ ≡ A₂ → Γ ⊢ e : A₁ → Γ ⊢ e : A₂
   univ_defInv : Γ ⊢ .sort u ≡ .sort v → u ≈ v
+  forallE_defInv : Γ ⊢ .forallE A B ≡ .forallE A' B' → Γ ⊢ A ≡ A' ∧ A::Γ ⊢ B ≡ B'
+
+theorem Typing.IsDefEq.weakN {TY : Typing} (W : Ctx.LiftN n k Γ Γ') :
+    TY.IsDefEq Γ e1 e2 → TY.IsDefEq Γ' (e1.liftN n k) (e2.liftN n k) := (TY.isDefEq_weakN_iff W).2
+theorem Typing.HasType.weakN {TY : Typing} (W : Ctx.LiftN n k Γ Γ') :
+    TY.HasType Γ e A → TY.HasType Γ' (e.liftN n k) (A.liftN n k) := (TY.hasType_weakN_iff W).2
 
 end
 
@@ -126,36 +155,42 @@ set_option hygiene false
 variable (TY : Typing)
 local notation:65 Γ " ⊢ " e " : " A:30 => TY.HasType Γ e A
 local notation:65 Γ " ⊢ " e1 " ≡ " e2:30 => TY.IsDefEq Γ e1 e2
-local notation:65 Γ " ⊢ " e1 " ≣ " e2:30 => NormalEq Γ e1 e2
+local notation:65 Γ " ⊢ " e1 " ≡ₚ " e2:30 => NormalEq Γ e1 e2
 
 inductive NormalEq : List VExpr → VExpr → VExpr → Prop where
-  | refl : Γ ⊢ e : A → Γ ⊢ e ≣ e
-  | sortDF : l₁.WF TY.univs → l₂.WF TY.univs → l₁ ≈ l₂ → Γ ⊢ .sort l₁ ≣ .sort l₂
+  | refl : Γ ⊢ e : A → Γ ⊢ e ≡ₚ e
+  | sortDF : l₁.WF TY.univs → l₂.WF TY.univs → l₁ ≈ l₂ → Γ ⊢ .sort l₁ ≡ₚ .sort l₂
+  | constDF :
+    TY.env.constants c = some (some ci) →
+    (∀ l ∈ ls, l.WF TY.univs) →
+    (∀ l ∈ ls', l.WF TY.univs) →
+    ls.length = ci.uvars →
+    List.Forall₂ (· ≈ ·) ls ls' →
+    Γ ⊢ .const c ls ≡ₚ .const c ls'
   | appDF :
     Γ ⊢ f₁ : .forallE A B → Γ ⊢ f₂ : .forallE A B →
     Γ ⊢ a₁ : A → Γ ⊢ a₂ : A →
-    Γ ⊢ f₁ ≣ f₂ → Γ ⊢ a₁ ≣ a₂ →
-    Γ ⊢ .app f₁ a₁ ≣ .app f₂ a₂
+    Γ ⊢ f₁ ≡ₚ f₂ → Γ ⊢ a₁ ≡ₚ a₂ →
+    Γ ⊢ .app f₁ a₁ ≡ₚ .app f₂ a₂
   | lamDF :
-    Γ ⊢ A : .sort u → Γ ⊢ A₁ ≡ A →
-    Γ ⊢ A₁ ≣ A₂ →
-    A::Γ ⊢ body₁ ≣ body₂ →
-    Γ ⊢ .lam A₁ body₁ ≣ .lam A₂ body₂
+    Γ ⊢ A : .sort u → Γ ⊢ A₁ ≡ A → Γ ⊢ A₁ ≡ₚ A₂ →
+    A::Γ ⊢ body₁ ≡ₚ body₂ →
+    Γ ⊢ .lam A₁ body₁ ≡ₚ .lam A₂ body₂
   | forallEDF :
-    Γ ⊢ A : .sort u → Γ ⊢ A₁ ≡ A → Γ ⊢ A₁ ≣ A₂ →
-    A::Γ ⊢ B₁ : .sort v → A::Γ ⊢ B₁ ≣ B₂ →
-    Γ ⊢ .forallE A₁ B₁ ≣ .forallE A₂ B₂
+    Γ ⊢ A : .sort u → Γ ⊢ A₁ ≡ A → Γ ⊢ A₁ ≡ₚ A₂ →
+    A::Γ ⊢ B₁ : .sort v → A::Γ ⊢ B₁ ≡ₚ B₂ →
+    Γ ⊢ .forallE A₁ B₁ ≡ₚ .forallE A₂ B₂
   | etaL :
     Γ ⊢ e' : .forallE A B →
-    A::Γ ⊢ e ≣ .app e'.lift (.bvar 0) →
-    Γ ⊢ .lam A e ≣ e'
+    A::Γ ⊢ e ≡ₚ .app e'.lift (.bvar 0) →
+    Γ ⊢ .lam A e ≡ₚ e'
   | etaR :
     Γ ⊢ e' : .forallE A B →
-    A::Γ ⊢ .app e'.lift (.bvar 0) ≣ e →
-    Γ ⊢ e' ≣ .lam A e
+    A::Γ ⊢ .app e'.lift (.bvar 0) ≡ₚ e →
+    Γ ⊢ e' ≡ₚ .lam A e
   | proofIrrel :
     Γ ⊢ p : .sort .zero → Γ ⊢ h : p → Γ ⊢ h' : p →
-    Γ ⊢ h ≣ h'
+    Γ ⊢ h ≡ₚ h'
 
 end
 
@@ -164,6 +199,7 @@ theorem NormalEq.defeq (H : NormalEq TY Γ e1 e2) : TY.IsDefEq Γ e1 e2 := by
   | refl h => exact TY.refl h
   | sortDF h1 h2 h3 => exact TY.sortDF h1 h2 h3
   | appDF hf₁ _ ha₁ _ _ _ ih1 ih2 => exact TY.appDF hf₁ ih1 ha₁ ih2
+  | constDF h1 h2 h3 h4 h5 => exact TY.constDF h1 h2 h3 h4 h5
   | lamDF hA hA₁ _ _ ihA ihB =>
     have ⟨_, hB⟩ := TY.has_type ihB
     exact TY.trans (TY.symm <| TY.lamDF hA (TY.symm hA₁) (TY.refl hB))
@@ -181,10 +217,12 @@ theorem NormalEq.defeq (H : NormalEq TY Γ e1 e2) : TY.IsDefEq Γ e1 e2 := by
     exact TY.trans (TY.symm (TY.eta h1)) (TY.lamDF hA (TY.refl hA) ih)
   | proofIrrel h1 h2 h3 => exact TY.proofIrrel h1 h2 h3
 
-theorem NormalEq.symm {env : VEnv} (H : NormalEq TY Γ e1 e2) : NormalEq TY Γ e2 e1 := by
+theorem NormalEq.symm (H : NormalEq TY Γ e1 e2) : NormalEq TY Γ e2 e1 := by
   induction H with
   | refl h => exact .refl h
   | sortDF h1 h2 h3 => exact .sortDF h2 h1 h3.symm
+  | constDF h1 h2 h3 h4 h5 =>
+    exact .constDF h1 h3 h2 (h5.length_eq.symm.trans h4) (h5.flip.imp (fun _ _ h => h.symm))
   | appDF h1 h2 h3 h4 _ _ ih1 ih2 => exact .appDF h2 h1 h4 h3 ih1 ih2
   | lamDF h1 h2 _ _ ih1 ih2 => exact .lamDF h1 (TY.trans ih1.defeq h2) ih1 ih2
   | forallEDF h1 h2 _ h4 h5 ih1 ih2 =>
@@ -193,43 +231,207 @@ theorem NormalEq.symm {env : VEnv} (H : NormalEq TY Γ e1 e2) : NormalEq TY Γ e
   | etaR h1 _ ih => exact .etaL h1 ih
   | proofIrrel h1 h2 h3 => exact .proofIrrel h1 h3 h2
 
-variable (TY : Typing) in
-theorem NormalEq.trans
-    (H1 : NormalEq TY Γ e1 e2) (H2 : NormalEq TY Γ e2 e3) :
-    NormalEq TY Γ e1 e3 := by
-  sorry
-  -- induction id H1 generalizing e3 with
-  -- | refl => exact H2
-  -- | proofIrrel l1 l2 l3 =>
-  --   induction H2 with
-  --   | refl => exact H1
-  --   | proofIrrel r1 r2 r3 =>
-  --     exact .proofIrrel l1 l2 (TY.defeq_r (TY.uniq r2 l3) r3)
-  --   | sortDF r1 =>
-  --     have hu := TY.sort_inv l3
-  --     have := TY.defeq_l (TY.uniq l3 (TY.sort hu)) l1
-  --     cases VLevel.equiv_def.1 (TY.univ_defInv <| TY.uniq this (TY.sort hu)) []
-  --   | appDF r1 r2 =>
+theorem NormalEq.weakN (W : Ctx.LiftN n k Γ Γ') (H : NormalEq TY Γ e1 e2) :
+    NormalEq TY Γ' (e1.liftN n k) (e2.liftN n k) := by
+  induction H generalizing k Γ' with
+  | refl h => refine .refl (h.weakN W)
+  | sortDF h1 h2 h3 => exact .sortDF h1 h2 h3
+  | constDF h1 h2 h3 h4 h5 => exact .constDF h1 h2 h3 h4 h5
+  | appDF h1 h2 h3 h4 _ _ ih1 ih2 =>
+    exact .appDF (h1.weakN W) (h2.weakN W) (h3.weakN W) (h4.weakN W) (ih1 W) (ih2 W)
+  | lamDF h1 h2 _ _ ih1 ih2 =>
+    exact .lamDF (h1.weakN W) (h2.weakN W) (ih1 W) (ih2 W.succ)
+  | forallEDF h1 h2 _ h4 _ ih1 ih2 =>
+    exact .forallEDF (h1.weakN W) (h2.weakN W) (ih1 W) (h4.weakN W.succ) (ih2 W.succ)
+  | etaL h1 _ ih =>
+    refine .etaL (h1.weakN W) ?_
+    have := ih W.succ
+    simp [liftN] at this; rwa [lift_liftN']
+  | etaR h1 _ ih =>
+    refine .etaR (h1.weakN W) ?_
+    have := ih W.succ
+    simp [liftN] at this; rwa [lift_liftN']
+  | proofIrrel h1 h2 h3 =>
+    exact .proofIrrel (h1.weakN W) (h2.weakN W) (h3.weakN W)
 
-  --     have hu := TY.sort_inv l3
-  --     have := TY.defeq_l (TY.uniq l3 (TY.sort hu)) l1
-  --     cases VLevel.equiv_def.1 (TY.univ_defInv <| TY.uniq this (TY.sort hu)) []
-  -- | sortDF l1 l2 l3 l4 l5 =>
-  --   cases H2 with
-  --   | refl => exact H1
-  --   | proofIrrel r1 r2 r3 => exact .proofIrrel r1 (H1.defeq henv hΓ).hasType.1 r3
-  --   | sortDF r1 r2 r3 r4 r5 => exact .sortDF l1 r2 l3 l4 r5
-  -- | @appDF _ a₁ a A a₂ f₁ f₂ B l1 l2 _ _ ihl1 ihl2 =>
-  --   generalize eq : inst B a = i at H2
-  --   cases H2 with
-  --   | refl => exact eq ▸ H1
-  --   | proofIrrel r1 r2 r3 => subst eq; exact .proofIrrel r1 (H1.defeq henv hΓ).hasType.1 r3
-  --   | @appDF _ a₁' a' A' a₂' f₁' f₂' B' r1 r2 ihr1 ihr2 =>
-  --     have := ihl1 hΓ _ ihr1
-  --     exact .appDF _ _ _ _
-  --   | etaR r1 ihr1 =>
-  --     exact .appDF _ _ _ _
-  -- | lamDF h1 h2 _ _ ih1 ih2 => exact .lamDF h2 h1 ih1 ih2
-  -- | forallEDF h1 h2 _ _ ih1 ih2 => exact .forallEDF h2 h1 ih1 ih2
-  -- | etaL h1 _ ih => exact .etaR h1 ih
-  -- | etaR h1 _ ih => exact .etaL h1 ih
+variable (TY : Typing) in
+theorem NormalEq.defeqDFC (W : IsDefEqCtx TY.IsDefEq Γ₀ Γ₁ Γ₂)
+    (H : NormalEq TY Γ₁ e1 e2) : NormalEq TY Γ₂ e1 e2 := by
+  induction H generalizing Γ₂ with
+  | refl h => refine .refl (TY.hasType_DFC W h)
+  | sortDF h1 h2 h3 => exact .sortDF h1 h2 h3
+  | constDF h1 h2 h3 h4 h5 => exact .constDF h1 h2 h3 h4 h5
+  | appDF h1 h2 h3 h4 _ _ ih1 ih2 =>
+    exact .appDF (TY.hasType_DFC W h1) (TY.hasType_DFC W h2)
+      (TY.hasType_DFC W h3) (TY.hasType_DFC W h4) (ih1 W) (ih2 W)
+  | lamDF h1 h2 _ _ ih1 ih2 =>
+    exact .lamDF (TY.hasType_DFC W h1) (TY.isDefEq_DFC W h2) (ih1 W) (ih2 (W.succ (TY.refl h1)))
+  | forallEDF h1 h2 _ h4 _ ih1 ih2 =>
+    exact .forallEDF (TY.hasType_DFC W h1) (TY.isDefEq_DFC W h2) (ih1 W)
+      (TY.hasType_DFC (W.succ (TY.refl h1)) h4) (ih2 (W.succ (TY.refl h1)))
+  | etaL h1 _ ih =>
+    have ⟨_, _, h2, _⟩ := let ⟨_, h⟩ := TY.is_type h1; TY.forallE_inv h
+    refine .etaL (TY.hasType_DFC W h1) (ih (W.succ (TY.refl h2)))
+  | etaR h1 _ ih =>
+    have ⟨_, _, h2, _⟩ := let ⟨_, h⟩ := TY.is_type h1; TY.forallE_inv h
+    refine .etaR (TY.hasType_DFC W h1) (ih (W.succ (TY.refl h2)))
+  | proofIrrel h1 h2 h3 =>
+    exact .proofIrrel (TY.hasType_DFC W h1)
+      (TY.hasType_DFC W h2) (TY.hasType_DFC W h3)
+
+theorem NormalEq.defeq_l (W : TY.IsDefEq Γ A A') (H : NormalEq TY (A::Γ) e1 e2) :
+    NormalEq TY (A'::Γ) e1 e2 := defeqDFC TY (.succ .zero W) H
+
+theorem NormalEq.weakN_inv_DFC (W : Ctx.LiftN n k Γ Γ₂) (W₂ : IsDefEqCtx TY.IsDefEq Γ₀ Γ₁ Γ₂)
+    (H : NormalEq TY Γ₁ (e1.liftN n k) (e2.liftN n k)) : NormalEq TY Γ e1 e2 := by
+  generalize eq1 : e1.liftN n k = e1' at H
+  generalize eq2 : e2.liftN n k = e2' at H
+  induction H generalizing Γ Γ₂ e1 e2 k with
+  | refl h =>
+    cases eq2; cases liftN_inj.1 eq1
+    have ⟨_, h'⟩ := TY.hasTypeU_weakN_inv W (TY.hasType_DFC W₂ h)
+    exact .refl h'
+  | sortDF h1 h2 h3 =>
+    cases e1 <;> cases eq1
+    cases e2 <;> cases eq2
+    exact .sortDF h1 h2 h3
+  | constDF h1 h2 h3 h4 h5 =>
+    cases e1 <;> cases eq1
+    cases e2 <;> cases eq2
+    exact .constDF h1 h2 h3 h4 h5
+  | appDF h1 h2 h3 h4 _ _ ih1 ih2 =>
+    cases e1 <;> cases eq1
+    cases e2 <;> cases eq2
+    replace h1 := TY.hasType_DFC W₂ h1
+    replace h2 := TY.hasType_DFC W₂ h2
+    replace h3 := TY.hasType_DFC W₂ h3
+    replace h4 := TY.hasType_DFC W₂ h4
+    have ⟨_, _, l1, l2⟩ :=
+      let ⟨_, h⟩ := TY.hasTypeU_weakN_inv W (TY.app h1 h3) (e := .app ..); TY.app_inv h
+    have ⟨_, _, r1, r2⟩ :=
+      let ⟨_, h⟩ := TY.hasTypeU_weakN_inv W (TY.app h2 h4) (e := .app ..); TY.app_inv h
+    have := (TY.isDefEq_weakN_iff W).1
+      (TY.trans (TY.uniq (l1.weakN W) h1) (TY.uniq h2 (r1.weakN W)))
+    exact .appDF (TY.defeq_r this l1) r1
+      (TY.defeq_r (TY.forallE_defInv this).1 l2) r2 (ih1 W W₂ rfl rfl) (ih2 W W₂ rfl rfl)
+  | lamDF h1 h2 _ _ ih1 ih2 =>
+    cases e1 <;> cases eq1
+    cases e2 <;> cases eq2
+    have := (TY.hasType_weakN_iff (A := .sort ..) W).1 <|
+      TY.hasType_DFC W₂ (TY.defeq_l (TY.symm h2) h1)
+    exact .lamDF this (TY.refl this) (ih1 W W₂ rfl rfl) (ih2 W.succ (W₂.succ (TY.symm h2)) rfl rfl)
+  | forallEDF h1 h2 _ h4 _ ih1 ih2 =>
+    cases e1 <;> cases eq1
+    cases e2 <;> cases eq2
+    replace h4 := (TY.hasType_weakN_iff (A := .sort ..) W.succ).1 <|
+      TY.hasType_DFC (W₂.succ (TY.symm h2)) h4
+    have := (TY.hasType_weakN_iff (A := .sort ..) W).1 <|
+      TY.hasType_DFC W₂ (TY.defeq_l (TY.symm h2) h1)
+    exact .forallEDF this (TY.refl this)
+      (ih1 W W₂ rfl rfl) h4 (ih2 W.succ (W₂.succ (TY.symm h2)) rfl rfl)
+  | etaL h1 _ ih =>
+    cases e1 <;> cases eq1
+    subst eq2
+    have ⟨_, _, hA, hB⟩ := let ⟨_, h⟩ := TY.is_type h1; TY.forallE_inv h
+    have h1' := TY.hasType_DFC W₂ h1
+    have hA' := TY.hasType_DFC W₂ hA
+    have hB' := TY.hasType_DFC (W₂.succ (TY.refl hA)) hB
+    have := TY.app (h1'.weakN .one) (TY.bvar .zero)
+    rw [instN_bvar0, ← lift, lift_liftN',
+      ← show liftN n (.bvar 0) (k+1) = bvar 0 by simp [liftN],
+      ← liftN] at this
+    have ⟨C, hC⟩ := TY.hasTypeU_weakN_inv W.succ this
+    have := (TY.hasType_weakN_iff (A := .forallE ..) W).1 <|
+      TY.defeq_r (TY.forallEDF hA' (TY.refl hA') hB' (TY.uniq this (hC.weakN W.succ))) h1'
+    refine .etaL this (ih W.succ (W₂.succ (TY.refl hA)) rfl (by simp [liftN, lift_liftN']))
+  | etaR h1 _ ih =>
+    subst eq1
+    cases e2 <;> cases eq2
+    have ⟨_, _, hA, hB⟩ := let ⟨_, h⟩ := TY.is_type h1; TY.forallE_inv h
+    have h1' := TY.hasType_DFC W₂ h1
+    have hA' := TY.hasType_DFC W₂ hA
+    have hB' := TY.hasType_DFC (W₂.succ (TY.refl hA)) hB
+    have := TY.app (h1'.weakN .one) (TY.bvar .zero)
+    rw [instN_bvar0, ← lift, lift_liftN',
+      ← show liftN n (.bvar 0) (k+1) = bvar 0 by simp [liftN],
+      ← liftN] at this
+    have ⟨C, hC⟩ := TY.hasTypeU_weakN_inv W.succ this
+    have := (TY.hasType_weakN_iff (A := .forallE ..) W).1 <|
+      TY.defeq_r (TY.forallEDF hA' (TY.refl hA') hB' (TY.uniq this (hC.weakN W.succ))) h1'
+    refine .etaR this (ih W.succ (W₂.succ (TY.refl hA)) (by simp [liftN, lift_liftN']) rfl)
+  | proofIrrel h1 h2 h3 =>
+    subst eq1; subst eq2
+    have h1' := TY.hasType_DFC W₂ h1
+    have h2' := TY.hasType_DFC W₂ h2
+    have h3' := TY.hasType_DFC W₂ h3
+    have ⟨_, h⟩ := TY.hasTypeU_weakN_inv W h2'
+    have hw := TY.uniq h2' (h.weakN W)
+    exact .proofIrrel
+      ((TY.hasType_weakN_iff (A := .sort ..) W).1 (TY.defeq_l hw h1'))
+      ((TY.hasType_weakN_iff W).1 (TY.defeq_r hw h2'))
+      ((TY.hasType_weakN_iff W).1 (TY.defeq_r hw h3'))
+
+theorem NormalEq.weakN_iff (W : Ctx.LiftN n k Γ Γ') :
+    NormalEq TY Γ' (e1.liftN n k) (e2.liftN n k) ↔ NormalEq TY Γ e1 e2 :=
+  ⟨fun H => H.weakN_inv_DFC W .zero, fun H => H.weakN W⟩
+
+private def meas : VExpr → Nat
+  | .app f a
+  | .forallE f a => meas f + meas a + 1
+  | .bvar _ | .const .. | .sort _ => 0
+  | .lam A e => meas A + meas e + 3
+
+private theorem meas_liftN : meas (e.liftN n k) = meas e := by
+  induction e generalizing k <;> simp [*, meas]
+private theorem meas_lift : meas e.lift = meas e := meas_liftN
+
+variable (TY : Typing) in
+attribute [local simp] meas meas_lift in
+theorem NormalEq.trans : NormalEq TY Γ e1 e2 → NormalEq TY Γ e2 e3 → NormalEq TY Γ e1 e3
+  | .sortDF l1 _ l3, .sortDF r1 r2 r3 => .sortDF l1 r2 (l3.trans r3)
+  | .constDF l1 l2 _ l4 l5, .constDF _ _ r3 r4 r5 =>
+    .constDF l1 l2 r3 l4 (l5.trans (fun _ _ _ h1 => h1.trans) r5)
+  | .appDF l1 l2 l3 l4 l5 l6, .appDF r1 r2 r3 r4 r5 r6 =>
+    .appDF l1 (TY.defeq_r (TY.uniq r1 l2) r2) l3
+      (TY.defeq_r (TY.uniq r3 l4) r4) (NormalEq.trans l5 r5) (NormalEq.trans l6 r6)
+  | .lamDF l1 l2 l3 l4, .lamDF _ r2 r3 r4 =>
+    have r4' := r4.defeq_l (TY.trans (TY.symm (TY.trans l3.defeq r2)) l2)
+    .lamDF l1 l2 (NormalEq.trans l3 r3) (NormalEq.trans l4 r4')
+  | .forallEDF l1 l2 l3 l4 l5, .forallEDF _ r2 r3 r4 r5 =>
+    have r5' := r5.defeq_l (TY.trans (TY.symm (TY.trans l3.defeq r2)) l2)
+    .forallEDF l1 l2 (NormalEq.trans l3 r3) l4 (NormalEq.trans l5 r5')
+  | .etaR l1 ih, .lamDF _ r2 r3 r4 =>
+    have ⟨_, _, hA, hB⟩ := let ⟨_, h⟩ := TY.is_type l1; TY.forallE_inv h
+    .etaR (TY.defeq_r (TY.forallEDF hA r3.defeq hB (TY.refl hB)) l1)
+      (NormalEq.trans (ih.defeq_l r3.defeq) (r4.defeq_l (TY.trans (TY.symm r2) r3.defeq)))
+  | .lamDF _ l2 l3 l4, .etaL r1 ih =>
+    have ⟨_, _, hA, hB⟩ := let ⟨_, h⟩ := TY.is_type r1; TY.forallE_inv h
+    .etaL (TY.defeq_r (TY.forallEDF hA l3.symm.defeq hB (TY.refl hB)) r1)
+      (NormalEq.trans (l4.defeq_l (TY.symm l2)) (ih.defeq_l l3.symm.defeq))
+  | H1@(.etaR l1 ihl), .etaL r1 ihr => by
+    have := NormalEq.trans ihl ihr
+    generalize eq : e1.lift = e1' at this
+    have ⟨_, _, hA, _⟩ := let ⟨_, h⟩ := TY.is_type l1; TY.forallE_inv h
+    cases this with first | cases eq | cases liftN_inj.1 eq
+    | refl h => exact .refl r1
+    | proofIrrel h1 h2 h3 =>
+      refine .proofIrrel (TY.defeq_r ?_ (TY.forallE hA h1))
+        (TY.defeq_l (TY.eta l1) (TY.lam hA h2)) (TY.defeq_l (TY.eta r1) (TY.lam hA h3))
+      have hw := let ⟨_, h⟩ := TY.is_type hA; TY.sort_inv h
+      exact TY.sortDF ⟨hw, ⟨⟩⟩ ⟨⟩ rfl
+    | appDF _ _ _ _ ih => exact (NormalEq.weakN_iff .one).1 ih
+  | .refl h, H2 => H2
+  | .proofIrrel l1 l2 l3, H2 => .proofIrrel l1 l2 (TY.defeq_l H2.defeq l3)
+  | .etaL l1 ih, H2 => by
+    refine .etaL (TY.defeq_l H2.defeq l1) (NormalEq.trans ih ?_)
+    exact .appDF (l1.weakN .one)
+      ((TY.defeq_l H2.defeq l1).weakN .one) (TY.bvar .zero) (TY.bvar .zero)
+      (.weakN .one H2) (.refl (TY.bvar .zero))
+  | H1, .refl _ => H1
+  | H1, .etaR r1 ih => by
+    refine .etaR (TY.defeq_l H1.symm.defeq r1) (NormalEq.trans ?_ ih)
+    refine .appDF ((TY.defeq_l H1.symm.defeq r1).weakN .one)
+      (r1.weakN .one) (TY.bvar .zero) (TY.bvar .zero)
+      (.weakN .one H1) (.refl (TY.bvar .zero))
+  | H1, .proofIrrel h1 h2 h3 => .proofIrrel h1 (TY.defeq_l H1.symm.defeq h2) h3
+termination_by meas e1 + meas e2 + meas e3
